sha/verif_hmacNK_update.v
@@ -36,12 +36,13 @@ assert (FC_i_ctx: field_compatible t_struct_hmac_ctx_st [StructField _i_ctx] c).
  {red in FC_c. red. intuition.  constructor. trivial. right; left. reflexivity. }
 unfold_data_at 1%nat.
 rewrite (field_at_data_at  _ _ [StructField _i_ctx]).
-rewrite (field_at_data_at _ _ [StructField _md_ctx]).   
-unfold field_address. rewrite if_true by trivial. rewrite if_true by trivial.
+rewrite (field_at_data_at _ _ [StructField _md_ctx]).  
+rewrite field_address_offset by auto with field_compatible.
+rewrite field_address_offset by auto with field_compatible.
 simpl @nested_field_type.
 make_Vptr c.
 simpl. rewrite Int.add_zero.
-Time forward_call (ctx, data, Vptr b i, d, Tsh, len, kv) s. (*12.7 secs*) 
+Time forward_call (ctx, data, Vptr b i, d, Tsh, len, kv) s. (*17.6 secs*) 
  (*Issue: the forward_call takes ca 50secs in newComCert, instead of 6secs in Master, 
    no matter wther the field_at_data_at stuff s done outside of the call or inside.
    Resolved (11/4/15): with the faster canceler, now 12.5 sec.
@@ -70,9 +71,10 @@ unfold_data_at 3%nat.
 destruct ST as [ST1 [ST2 ST3]]. simpl in *.
 rewrite (field_at_data_at _ _ [StructField _i_ctx]).
 rewrite (field_at_data_at _ _ [StructField _md_ctx]).
-unfold field_address. rewrite !if_true by eauto.
+rewrite field_address_offset by auto with field_compatible.
+rewrite field_address_offset by auto with field_compatible.
 simpl. rewrite Int.add_zero.
    change (@data_block spec_sha.CompSpecs Tsh data data')
      with (@data_block CompSpecs Tsh data data').
-Time cancel. (*0.75 *)
-Time Qed. (*22*)
+Time cancel. (*0.5 *)
+Time Qed. (*22.8*)
